Cslib.lean
@@ -371,6 +371,9 @@ public import Cslib.Logics.Propositional.ProofSystem.Instances
 public import Cslib.Logics.Propositional.ProofSystem.IntMinInstances
 public import Cslib.Logics.Propositional.Semantics.Algebra
 public import Cslib.Logics.Propositional.Semantics.Algebra.Bridge
+public import Cslib.Logics.Propositional.Semantics.Algebra.Completeness
+public import Cslib.Logics.Propositional.Semantics.Algebra.Conservative
+public import Cslib.Logics.Propositional.Semantics.Algebra.Lindenbaum
 public import Cslib.Logics.Propositional.Semantics.Algebra.Soundness
 public import Cslib.Logics.Propositional.Semantics.Bool
 public import Cslib.Logics.Propositional.Semantics.Kripke
